Prove that DCVE maintains renamedApart.

theories/DCVE.v
@@ -1,46 +1,54 @@
-Require Import Util AllInRel MapDefined IL Rename RenameApart Sim Status Annotation.
+Require Import Util AllInRel MapDefined IL Sim Status Annotation.
+Require Import Rename RenamedApart RenamedApart_Liveness.
 Require UCE DVE.
-Require ReachabilityAnalysis ReachabilityAnalysisCorrect.
-Require TrueLiveness LivenessAnalysis LivenessAnalysisCorrect.
+Require Import Reachability ReachabilityAnalysis ReachabilityAnalysisCorrect.
+Require Import TrueLiveness.
+Require LivenessAnalysis LivenessAnalysisCorrect.
 
 Arguments sim S {H} S' {H0} r t _ _.
 
-Definition DCVE i (s:IL.stmt) : stmt * ann (set var) :=
-  let uc := ReachabilityAnalysis.reachabilityAnalysis s in
+Notation "'co_s' x" := (fst (fst x)) (at level 50).
+Notation "'co_lv' x" := (snd (fst x)) (at level 50).
+Notation "'co_ra' x" := (snd x) (at level 50).
+
+Definition DCVE i (s:IL.stmt) (ra:ann (⦃var⦄ * ⦃var⦄)) : stmt * ann ⦃var⦄ * ann (⦃var⦄ * ⦃var⦄) :=
+  let uc := reachabilityAnalysis s in
   let s_uce := UCE.compile nil s uc in
+  let ra_uce := UCE.compile_renamedApart s ra uc in
   let tlv := LivenessAnalysis.livenessAnalysis i s_uce in
   let s_dve := DVE.compile nil s_uce tlv in
-  (s_dve, DVE.compile_live s_uce tlv ∅).
+  let ra_dve := DVE.compile_renamedApart s_uce tlv ra_uce (fst (getAnn ra_uce)) in
+  (s_dve, DVE.compile_live s_uce tlv ∅, ra_dve).
 
-Lemma DCVE_live i (ili:IL.stmt) (PM:LabelsDefined.paramsMatch ili nil)
-  : Liveness.live_sound i nil nil (fst (DCVE i ili)) (snd (DCVE i ili)).
+Lemma DCVE_live i (ili:IL.stmt) (PM:LabelsDefined.paramsMatch ili nil) ra
+  : Liveness.live_sound i nil nil (co_s (DCVE i ili ra)) (co_lv (DCVE i ili ra)).
 Proof.
   unfold DCVE. simpl.
   eapply (@DVE.dve_live _ nil nil).
   eapply @LivenessAnalysisCorrect.correct; eauto.
   eapply (@UCE.UCE_paramsMatch nil nil); eauto.
-  eapply Reachability.reachability_SC_S, ReachabilityAnalysisCorrect.correct; eauto.
-  eapply ReachabilityAnalysisCorrect.reachabilityAnalysis_getAnn.
+  eapply reachability_SC_S, correct; eauto.
+  eapply reachabilityAnalysis_getAnn.
 Qed.
 
-Lemma DCVE_noUC i ili (PM:LabelsDefined.paramsMatch ili nil)
-  : LabelsDefined.noUnreachableCode LabelsDefined.isCalled (fst (DCVE i ili)).
+Lemma DCVE_noUC i ili (PM:LabelsDefined.paramsMatch ili nil) ra
+  : LabelsDefined.noUnreachableCode LabelsDefined.isCalled (co_s (DCVE i ili ra)).
 Proof.
   intros. subst. simpl.
   eapply LabelsDefined.noUnreachableCode_mono.
   - eapply (@DVE.DVE_noUnreachableCode _ nil nil).
     + eapply @LivenessAnalysisCorrect.correct; eauto.
       eapply (@UCE.UCE_paramsMatch nil nil); eauto.
-      * eapply Reachability.reachability_SC_S, ReachabilityAnalysisCorrect.correct; eauto.
-      * eapply ReachabilityAnalysisCorrect.reachabilityAnalysis_getAnn.
+      * eapply reachability_SC_S, correct; eauto.
+      * eapply reachabilityAnalysis_getAnn.
     + eapply UCE.UCE_noUnreachableCode.
-      * eapply ReachabilityAnalysisCorrect.correct; eauto.
-      * eapply ReachabilityAnalysisCorrect.reachabilityAnalysis_getAnn.
+      * eapply correct; eauto.
+      * eapply reachabilityAnalysis_getAnn.
   - eapply LabelsDefined.trueIsCalled_isCalled.
 Qed.
 
-Lemma DCVE_occurVars i s (PM:LabelsDefined.paramsMatch s nil)
-  : getAnn (snd (DCVE i s)) ⊆ occurVars s.
+Lemma DCVE_occurVars i s (PM:LabelsDefined.paramsMatch s nil) ra
+  : getAnn (co_lv (DCVE i s ra)) ⊆ occurVars s.
 Proof.
   simpl.
   rewrite DVE.compile_live_incl_empty; eauto.
@@ -48,71 +56,118 @@ Proof.
   eapply UCE.compile_occurVars.
   eapply @LivenessAnalysisCorrect.correct; eauto.
   eapply (@UCE.UCE_paramsMatch nil nil); eauto.
-  * eapply Reachability.reachability_SC_S, ReachabilityAnalysisCorrect.correct; eauto.
-  * eapply ReachabilityAnalysisCorrect.reachabilityAnalysis_getAnn.
+  * eapply reachability_SC_S, correct; eauto.
+  * eapply reachabilityAnalysis_getAnn.
 Qed.
 
-Lemma DCVE_correct_I (ili:IL.stmt) (E:onv val)
+Lemma DCVE_correct_I (ili:IL.stmt) (E:onv val) ra
   (PM:LabelsDefined.paramsMatch ili nil)
   : defined_on (IL.occurVars ili) E
-    -> sim I.state I.state bot3 Sim (nil, E, ili) (nil, E, fst (DCVE Liveness.Imperative ili)).
+    -> sim I.state I.state bot3 Sim (nil, E, ili) (nil, E, co_s (DCVE Liveness.Imperative ili ra)).
 Proof.
   intros. subst. unfold DCVE.
   simpl in *.
-  assert (Reachability.reachability Reachability.SoundAndComplete nil ili
-                                           (ReachabilityAnalysis.reachabilityAnalysis ili)). {
-    eapply ReachabilityAnalysisCorrect.correct; eauto.
+  assert (reachability SoundAndComplete nil ili
+                                           (reachabilityAnalysis ili)). {
+    eapply correct; eauto.
   }
-  assert (getAnn (ReachabilityAnalysis.reachabilityAnalysis ili)). {
-    eapply ReachabilityAnalysisCorrect.reachabilityAnalysis_getAnn.
+  assert (getAnn (reachabilityAnalysis ili)). {
+    eapply reachabilityAnalysis_getAnn.
   }
   assert (LabelsDefined.paramsMatch
-            (UCE.compile nil ili (ReachabilityAnalysis.reachabilityAnalysis ili)) nil). {
+            (UCE.compile nil ili (reachabilityAnalysis ili)) nil). {
     eapply (@UCE.UCE_paramsMatch nil nil); eauto.
   }
   assert (TrueLiveness.true_live_sound Liveness.Imperative nil nil
-   (UCE.compile nil ili (ReachabilityAnalysis.reachabilityAnalysis ili))
+   (UCE.compile nil ili (reachabilityAnalysis ili))
    (LivenessAnalysis.livenessAnalysis Liveness.Imperative
-      (UCE.compile nil ili (ReachabilityAnalysis.reachabilityAnalysis ili)))). {
+      (UCE.compile nil ili (reachabilityAnalysis ili)))). {
     eapply @LivenessAnalysisCorrect.correct; eauto.
   }
   eapply sim_trans with (S2:=I.state).
   eapply bisim_sim.
   eapply UCE.I.sim_UCE.
-  eapply Reachability.reachability_SC_S, ReachabilityAnalysisCorrect.correct; eauto.
-  eapply ReachabilityAnalysisCorrect.reachabilityAnalysis_getAnn.
+  eapply reachability_SC_S, correct; eauto.
+  eapply reachabilityAnalysis_getAnn.
   eapply DVE.I.sim_DVE; [ reflexivity | eapply LivenessAnalysisCorrect.correct; eauto ].
 Qed.
 
 
-Lemma DCVE_correct_F (ilf:IL.stmt) (E:onv val)
+Lemma DCVE_correct_F (ilf:IL.stmt) (E:onv val) ra
   (PM:LabelsDefined.paramsMatch ilf nil)
   : defined_on (IL.occurVars ilf) E
-    -> sim F.state F.state bot3 Sim (nil, E, ilf) (nil, E, fst (DCVE Liveness.Functional ilf)).
+    -> sim F.state F.state bot3 Sim (nil, E, ilf) (nil, E, co_s (DCVE Liveness.Functional ilf ra)).
 Proof.
   intros. subst. unfold DCVE.
   simpl in *.
-  assert (Reachability.reachability Reachability.SoundAndComplete nil ilf
-                                           (ReachabilityAnalysis.reachabilityAnalysis ilf)). {
-    eapply ReachabilityAnalysisCorrect.correct; eauto.
+  assert (reachability SoundAndComplete nil ilf
+                                           (reachabilityAnalysis ilf)). {
+    eapply correct; eauto.
   }
-  assert (getAnn (ReachabilityAnalysis.reachabilityAnalysis ilf)). {
-    eapply ReachabilityAnalysisCorrect.reachabilityAnalysis_getAnn.
+  assert (getAnn (reachabilityAnalysis ilf)). {
+    eapply reachabilityAnalysis_getAnn.
   }
   assert (LabelsDefined.paramsMatch
-            (UCE.compile nil ilf (ReachabilityAnalysis.reachabilityAnalysis ilf)) nil). {
+            (UCE.compile nil ilf (reachabilityAnalysis ilf)) nil). {
     eapply (@UCE.UCE_paramsMatch nil nil); eauto.
   }
   assert (TrueLiveness.true_live_sound Liveness.Imperative nil nil
-   (UCE.compile nil ilf (ReachabilityAnalysis.reachabilityAnalysis ilf))
+   (UCE.compile nil ilf (reachabilityAnalysis ilf))
    (LivenessAnalysis.livenessAnalysis Liveness.Imperative
-      (UCE.compile nil ilf (ReachabilityAnalysis.reachabilityAnalysis ilf)))). {
+      (UCE.compile nil ilf (reachabilityAnalysis ilf)))). {
     eapply @LivenessAnalysisCorrect.correct; eauto.
   }
   eapply sim_trans with (S2:=F.state).
   eapply bisim_sim.
   eapply UCE.F.sim_UCE.
-  eapply Reachability.reachability_SC_S, ReachabilityAnalysisCorrect.correct; eauto.
-  eapply ReachabilityAnalysisCorrect.reachabilityAnalysis_getAnn.
+  eapply reachability_SC_S, correct; eauto.
+  eapply reachabilityAnalysis_getAnn.
   eapply DVE.F.sim_DVE; [ reflexivity | eapply LivenessAnalysisCorrect.correct; eauto ].
+Qed.
+
+Definition compile_renamedApart i s ra :=
+  let ra' := (UCE.compile_renamedApart s ra (reachabilityAnalysis s)) in
+  DVE.compile_renamedApart (UCE.compile nil s (reachabilityAnalysis s))
+                           (LivenessAnalysis.livenessAnalysis i
+                                                              (UCE.compile nil s (reachabilityAnalysis s)))
+                           ra'
+                           (fst (getAnn ra')).
+
+Lemma DCVE_renamedApart i s ra (PM:LabelsDefined.paramsMatch s nil)
+  : renamedApart s ra
+    -> renamedApart (co_s (DCVE i s ra)) (co_ra (DCVE i s ra)).
+Proof.
+  intros. simpl.
+  assert (true_live_sound i nil nil (UCE.compile nil s (reachabilityAnalysis s))
+          (LivenessAnalysis.livenessAnalysis i (UCE.compile nil s (reachabilityAnalysis s)))). {
+    eapply @LivenessAnalysisCorrect.correct; eauto.
+    - eapply (@UCE.UCE_paramsMatch nil nil); eauto.
+      + eapply reachability_SC_S, correct; eauto.
+      + eapply reachabilityAnalysis_getAnn.
+  }
+  exploit (@LivenessAnalysisCorrect.correct i); eauto.
+  eapply (@DVE.DVE_renamedApart i nil nil); eauto.
+  - eapply UCE.UCE_renamedApart; eauto.
+    + eapply reachability_SC_S, correct; eauto.
+  - rewrite <- renamedApart_freeVars.
+    Focus 2.
+    eapply UCE.UCE_renamedApart; eauto.
+    eapply reachability_SC_S, correct; eauto.
+    + rewrite DVE.DVE_freeVars; eauto.
+      destruct i; eauto using TrueLiveness.true_live_sound_overapproximation_F.
+      * eapply TrueLiveness.true_live_sound_overapproximation_F.
+        eapply renamedApart_true_live_imperative_is_functional; eauto.
+        -- eapply UCE.UCE_renamedApart; eauto.
+           ++ eapply reachability_SC_S, correct; eauto.
+        -- eapply UCE.UCE_noUnreachableCode; eauto.
+           ++ eapply correct; eauto.
+           ++ eapply reachabilityAnalysis_getAnn.
+        -- eapply LivenessAnalysisCorrect.livenessAnalysis_renamedApart_incl.
+           ++ eapply UCE.UCE_renamedApart; eauto.
+             ** eapply reachability_SC_S, correct; eauto.
+           ++ eapply (@paramsMatch_labelsDefined _ nil).
+             eapply (@UCE.UCE_paramsMatch nil nil); eauto.
+             ** eapply reachability_SC_S, correct; eauto.
+             ** eapply reachabilityAnalysis_getAnn.
+        -- isabsurd.
 Qed.
